matching-logic/src/Theories/Sorts_ProofSystem.v
@@ -36,6 +36,349 @@ Open Scope list_scope.
 
 Set Printing All.
 
+
+  (* TODO: derive congruence_app with this *)
+  Lemma congruence_app1 {Σ : Signature} Γ ψ1 ψ2 p q E i
+    (wfψ1: well_formed ψ1)
+    (wfψ2: well_formed ψ2)
+    (wfp: well_formed p)
+    (wfq: well_formed q)
+    (pf₁: Γ ⊢i ψ1^[[evar: E ↦ p]] ---> ψ1^[[evar: E ↦ q]] using i)
+    (pf₂: Γ ⊢i ψ2^[[evar: E ↦ p]] ---> ψ2^[[evar: E ↦ q]] using i)
+    :
+    (Γ ⊢i (ψ1^[[evar: E ↦ p]]) $ (ψ2^[[evar: E ↦ p]]) ---> (ψ1^[[evar: E ↦ q]]) $ (ψ2^[[evar: E ↦ q]]) using i).
+  Proof.
+    remember (well_formed_free_evar_subst_0 E _ _ wfp wfψ1) as Hwf1.
+    remember (well_formed_free_evar_subst_0 E _ _ wfq wfψ1) as Hwf2.
+    remember (well_formed_free_evar_subst_0 E _ _ wfp wfψ2) as Hwf3.
+    remember (well_formed_free_evar_subst_0 E _ _ wfq wfψ2) as Hwf4.
+    eapply syllogism_meta.
+    4: {
+      eapply Framing_right; auto. try_solve_pile.
+      apply pf₂.
+    }
+    1-3: wf_auto2.
+    eapply Framing_left; auto. try_solve_pile.
+  Qed.
+
+  (* TODO: overwrite with this *)
+  Lemma framing_left_under_tot_impl {Σ : Signature} {syntax : Definedness_Syntax.Syntax} Γ ψ phi1 phi2 psi x i:
+    well_formed ψ = true ->
+    well_formed phi1 = true ->
+    well_formed phi2 = true ->
+    well_formed psi = true ->
+    theory ⊆ Γ ->
+    x ∉ free_evars ψ ∪ free_evars psi ->
+    ProofInfoLe (ExGen := {[ev_x; x]}, SVSubst := ∅, KT := false, AKT := false) i ->
+    Γ ⊢i ⌊ ψ ⌋ ---> phi1 ---> phi2 using i->
+    Γ ⊢i ⌊ ψ ⌋ ---> (phi1 $ psi) ---> (phi2 $ psi) using i
+  .
+  Proof.
+    intros Hwfψ Hwfphi1 Hwfphi2 Hwfpsi HΓ HIn HPile H.
+    assert (S2: Γ ⊢i phi1 ---> (phi2 or ⌈ ! ψ ⌉) using i).
+    { toMLGoal.
+      { wf_auto2. }
+      mlAdd H as "H". mlIntro "Hphi1".
+      mlClassic (⌈ ! ψ ⌉) as "Hcl1" "Hcl2".
+      { wf_auto2. }
+      - mlRight. mlExact "Hcl1".
+      - mlLeft.
+        mlApply "H".
+        mlSplitAnd.
+        { mlExact "Hcl2". }
+        { mlExact "Hphi1". }
+    }
+
+    assert (S3: Γ ⊢i (⌈ ! ψ ⌉ $ psi) ---> ⌈ ! ψ ⌉ using i).
+    {
+      replace (⌈ ! ψ ⌉ $ psi)
+        with (subst_ctx (ctx_app_l AC_patt_defined psi ltac:(assumption)) (! ψ))
+        by reflexivity.
+      gapply (in_context_impl_defined _ _ _ x).
+      4: { wf_auto2. }
+      2: { exact HΓ. }
+      1: { assumption. }
+      set_solver.
+    }
+
+    assert (S4: Γ ⊢i (phi1 $ psi) ---> ((phi2 or ⌈ ! ψ ⌉) $ psi) using i).
+    {
+      unshelve (eapply Framing_left).
+      { wf_auto2. }
+      { try_solve_pile. }
+      { exact S2. }
+    }
+
+    assert (S5: Γ ⊢i (phi1 $ psi) ---> ((phi2 $ psi) or (⌈ ! ψ ⌉ $ psi)) using i).
+    {
+      pose proof (Htmp := prf_prop_or_iff Γ (ctx_app_l box psi ltac:(assumption)) phi2 (⌈! ψ ⌉)).
+      ospecialize* Htmp.
+      { wf_auto2. }
+      { wf_auto2. }
+      simpl in Htmp.
+      apply pf_iff_proj1 in Htmp.
+      3: { wf_auto2. }
+      2: { wf_auto2. }
+      eapply syllogism_meta.
+      5: {
+        gapply Htmp.
+        try_solve_pile.
+      }
+      4: { exact S4. }
+      all: wf_auto2.
+    }
+
+    assert (S6: Γ ⊢i ((phi2 $ psi) or (⌈ ! ψ ⌉ $ psi)) ---> ((phi2 $ psi) or (⌈ ! ψ ⌉)) using i).
+    {
+      toMLGoal.
+      { wf_auto2. }
+      mlIntro "H". mlAdd S3 as "S3".
+      mlClassic (phi2 $ psi) as "Hc1" "Hc2".
+      { wf_auto2. }
+      - mlLeft. mlExact "Hc1".
+      - mlRight. mlApply "S3". mlApply "H". mlExact "Hc2".
+    }
+
+    assert (S7: Γ ⊢i (phi1 $ psi) ---> ((phi2 $ psi)  or ⌈ ! ψ ⌉) using i).
+    {
+      toMLGoal.
+      { wf_auto2. }
+      mlAdd S5 as "S5".
+      mlAdd S6 as "S6".
+      mlIntro "H".
+      mlAssert ("Ha" : ((phi2 $ psi) or (⌈ ! ψ ⌉ $ psi))).
+      { wf_auto2. }
+      { mlApply "S5". mlExact "H". }
+      mlDestructOr "Ha" as "Ha1" "Ha2".
+      - mlLeft. mlExact "Ha1".
+      - mlApply "S6". mlRight. mlExact "Ha2".
+    }
+
+    toMLGoal.
+    { wf_auto2. }
+    mlIntro "H1".
+    mlIntro "H2".
+    mlAdd S7 as "S7".
+    mlAssert ("Ha" : (phi2 $ psi or ⌈ ! ψ ⌉)).
+    { wf_auto2. }
+    { mlApply "S7". mlExact "H2". }
+    mlDestructOr "Ha" as "Ha1" "Ha2".
+    { mlExact "Ha1". }
+    { mlAssert ("Ha'" : (phi2 $ psi or ⌈ ! ψ ⌉)).
+      { wf_auto2. }
+      { mlApply "S7". mlExact "H2". }
+      mlClassic (phi2 $ psi) as "Hc1" "Hc2".
+      { wf_auto2. }
+      { mlExact "Hc1". }
+      {
+        mlExFalso.
+        mlApply "H1".
+        mlExact "Ha2".
+      }
+    }
+  Defined.
+
+  (* TODO: overwrite with this *)
+  Lemma framing_right_under_tot_impl {Σ : Signature} {syntax : Definedness_Syntax.Syntax} Γ ψ phi1 phi2 psi x i:
+    well_formed ψ = true ->
+    well_formed phi1 = true ->
+    well_formed phi2 = true ->
+    well_formed psi = true ->
+    theory ⊆ Γ ->
+    x ∉ free_evars ψ ∪ free_evars psi ->
+    ProofInfoLe (ExGen := {[ev_x; x]}, SVSubst := ∅, KT := false, AKT := false) i ->
+    Γ ⊢i ⌊ ψ ⌋ ---> phi1 ---> phi2 using i->
+    Γ ⊢i ⌊ ψ ⌋ ---> (psi $ phi1) ---> (psi $ phi2) using i
+  .
+  Proof.
+    intros Hwfψ Hwfphi1 Hwfphi2 Hwfpsi HΓ HIn HPile H.
+    assert (S2: Γ ⊢i phi1 ---> (phi2 or ⌈ ! ψ ⌉) using i).
+    { toMLGoal.
+      { wf_auto2. }
+      mlAdd H as "H". mlIntro "Hphi1".
+      mlClassic (⌈ ! ψ ⌉) as "Hc1" "Hc2".
+      { wf_auto2. }
+      - mlRight. mlExact "Hc1".
+      - mlLeft.
+        mlApply "H".
+        mlSplitAnd.
+        { mlExact "Hc2". }
+        { mlExact "Hphi1". }
+    }
+
+    assert (S3: Γ ⊢i (psi $ ⌈ ! ψ ⌉) ---> ⌈ ! ψ ⌉ using i).
+    {
+      replace (psi $ ⌈ ! ψ ⌉)
+      with (subst_ctx (ctx_app_r psi AC_patt_defined ltac:(assumption)) (! ψ))
+        by reflexivity.
+      gapply (in_context_impl_defined _ _ _ x).
+      4: { wf_auto2. }
+      2: { exact HΓ. }
+      1: { assumption. }
+      set_solver.
+    }
+
+    assert (S4: Γ ⊢i (psi $ phi1) ---> (psi $ (phi2 or ⌈ ! ψ ⌉)) using i).
+    { 
+      unshelve (eapply Framing_right).
+      { wf_auto2. }
+      2: exact S2.
+      try_solve_pile.
+    }
+
+    assert (S5: Γ ⊢i (psi $ phi1) ---> ((psi $ phi2) or (psi $ ⌈ ! ψ ⌉)) using i).
+    {
+      pose proof (Htmp := prf_prop_or_iff Γ (ctx_app_r psi box ltac:(assumption)) phi2 (⌈! ψ ⌉)).
+      ospecialize* Htmp.
+      { wf_auto2. }
+      { wf_auto2. }
+      simpl in Htmp.
+      apply pf_iff_proj1 in Htmp.
+      2,3: wf_auto2.
+      eapply syllogism_meta.
+      5: gapply Htmp; try_solve_pile.
+      1-3: wf_auto2.
+      exact S4.
+    }
+
+    assert (S6: Γ ⊢i ((psi $ phi2) or (psi $ ⌈ ! ψ ⌉)) ---> ((psi $ phi2) or (⌈ ! ψ ⌉)) using i).
+    {
+      toMLGoal.
+      { wf_auto2. }
+      mlIntro "H1". mlAdd S3 as "S3".
+      mlClassic (psi $ phi2) as "Hc1" "Hc2".
+      { wf_auto2. }
+      - mlLeft. mlExact "Hc1".
+      - mlRight. mlApply "S3". mlApply "H1". mlExact "Hc2".
+    }
+
+    assert (S7: Γ ⊢i (psi $ phi1) ---> ((psi $ phi2)  or ⌈ ! ψ ⌉) using i).
+    {
+      toMLGoal.
+      { wf_auto2. }
+      mlAdd S5 as "S5". mlAdd S6 as "S6". mlIntro "H".
+      (* TODO: a tactic mlFeedImpl *)
+      mlAssert ("Ha" : ((psi $ phi2) or (psi $ ⌈ ! ψ ⌉))).
+      { wf_auto2. }
+      { mlApply "S5". mlExact "H". }
+      mlDestructOr "Ha" as "Ha1" "Ha2".
+      - mlLeft. mlExact "Ha1".
+      - mlApply "S6". mlRight. mlExact "Ha2".
+    }
+
+    toMLGoal.
+    { wf_auto2. }
+    mlIntro "H1".
+    mlIntro "H2".
+    mlAdd S7 as "S7".
+    mlAssert ("Ha" : (psi $ phi2 or ⌈ ! ψ ⌉)).
+    { wf_auto2. }
+    { mlApply "S7". mlExact "H2". }
+    mlDestructOr "Ha" as "Ha1" "Ha2".
+    { mlExact "Ha1". }
+    + mlAssert ("Ha'" : (psi $ phi2 or ⌈ ! ψ ⌉)).
+      { wf_auto2. }
+      { mlApply "S7". mlExact "H2". }
+      mlClassic (psi $ phi2) as "Hc1" "Hc2".
+      { wf_auto2. }
+      { mlExact "Hc1". }
+      {
+        mlExFalso.
+        mlApply "H1".
+        mlExact "Ha2".
+      }
+  Defined.
+
+  (* TODO: delete this *)
+  Lemma patt_equal_sym {Σ : Signature} {syntax : Definedness_Syntax.Syntax} Γ φ1 φ2 i:
+    theory ⊆ Γ ->
+    well_formed φ1 -> well_formed φ2 ->
+    ProofInfoLe BasicReasoning i ->
+    Γ ⊢i φ1 =ml φ2 ---> φ2 =ml φ1
+    using i.
+  Proof.
+    intros.
+    apply floor_monotonic; auto.
+    mlIntro. mlDestructAnd "0". mlSplitAnd; mlAssumption.
+  Qed.
+
+(*  eq-elim.0 $e #Substitution ph2 ph4 ph0 x $.   => ph2 = ph4[ph0/x]
+    eq-elim.1 $e #Substitution ph3 ph4 ph1 x $.   => ph3 = ph4[ph1/x]
+    eq-elim $a |- ( \imp ( \eq ph0 ph1 ) ( \imp ph2 ph3 ) ) $.
+                                                  => ph0 = ph1 -> ph2 -> ph3
+ *)
+Lemma equality_elimination_basic 
+  {Σ : Signature}
+  {sy : Definedness_Syntax.Syntax}
+  Γ φ1 φ2 C x
+  (HΓ : theory ⊆ Γ)
+  (WF1 : well_formed φ1)
+  (WF2 :  well_formed φ2)
+  (WFC : PC_wf C)
+  (Hfree : x ∉ free_evars φ1 ∪ free_evars φ2 ∪ free_evars (pcPattern C)) :
+(*   mu_free (pcPattern C) -> *)
+  Γ ⊢i (φ1 =ml φ2) --->
+    (emplace C φ1) ---> (emplace C φ2)
+  using (ExGen := {[ev_x; x]}, SVSubst := ∅, KT := false, AKT := false).
+Proof.
+  destruct C as [y φ4]. cbn in *.
+  assert (well_formed φ4) by wf_auto2. clear WFC.
+  remember (size' φ4) as sz.
+  assert (size' φ4 <= sz) by lia. clear Heqsz.
+  revert φ4 φ1 φ2 x Γ HΓ H0 H WF1 WF2 Hfree. induction sz; intros.
+  {
+    destruct φ4; simpl in H0; lia.
+  }
+  destruct φ4; simpl in *.
+  * case_match.
+    - subst.
+      mlIntro "H".
+      mlApplyMeta total_phi_impl_phi in "H".
+      2: set_solver.
+      2: wf_auto2.
+      mlDestructAnd "H".
+      mlAssumption.
+    - do 2 mlIntro. mlAssumption.
+  * do 2 mlIntro. mlAssumption.
+  * do 2 mlIntro. mlAssumption.
+  * do 2 mlIntro. mlAssumption.
+  * do 2 mlIntro. mlAssumption.
+  * mlIntro "H".
+    pose proof (IH1 := IHsz φ4_1 φ1 φ2 x Γ HΓ ltac:(lia) ltac:(wf_auto2) ltac:(wf_auto2) ltac:(wf_auto2) ltac:(set_solver)).
+    pose proof (IH2 := IHsz φ4_2 φ1 φ2 x Γ HΓ ltac:(lia) ltac:(wf_auto2) ltac:(wf_auto2) ltac:(wf_auto2) ltac:(set_solver)).
+    clear IHsz.
+    mlAssert ("H2" : (φ1 =ml φ2)). wf_auto2. mlAssumption.
+    eapply framing_left_under_tot_impl with (x := x) in IH1.
+    eapply framing_right_under_tot_impl with (x := x) in IH2.
+    mlApplyMeta IH1 in "H".
+    mlApplyMeta IH2 in "H2".
+    mlIntro "H0".
+    mlApply "H".
+    mlApply "H2".
+    mlAssumption.
+    5, 12: assumption.
+    6, 12: try_solve_pile.
+    1-4,6-9: wf_auto2.
+    clear -Hfree.
+    1-2: pose proof free_evars_free_evar_subst; set_solver.
+  * do 2 mlIntro. mlAssumption.
+  * mlIntro "H".
+    pose proof (IH1 := IHsz φ4_1 φ2 φ1 x Γ HΓ ltac:(lia) ltac:(wf_auto2) ltac:(wf_auto2) ltac:(wf_auto2) ltac:(set_solver)).
+    pose proof (IH2 := IHsz φ4_2 φ1 φ2 x Γ HΓ ltac:(lia) ltac:(wf_auto2) ltac:(wf_auto2) ltac:(wf_auto2) ltac:(set_solver)).
+    clear IHsz.
+    mlAssert ("H2" : (φ2 =ml φ1)). wf_auto2.
+    {
+      mlApplyMeta patt_equal_sym. mlAssumption. assumption.
+    }
+    mlApplyMeta IH1 in "H2".
+    mlApplyMeta IH2 in "H".
+    mlIntro "H0". mlIntro "S".
+    clear. mlApply "H". mlApply "H0". mlApply "H2". mlAssumption.
+  * 
+  *
+Qed.
+
+
 Local Lemma simplTest
   {Σ : Signature}
   {syntax : Sorts_Syntax.Syntax}
